Reduce number of assumes

examples/lowstar_permissions/Test.Array.fst
@@ -79,27 +79,25 @@ let read_write_with_sharing () : RST.RST unit
     (fun p -> R.(A.array_resource (fst p) <*> A.array_resource (snd p) <*> A.array_resource b1))
     (let f = fun _ -> A.split #FStar.UInt32.t b 1ul in f) //TODO: remove let binding
   in
-
+  let h = HST.get () in
+   let full = R.(A.array_resource b_first <*> A.array_resource b_second <*> A.array_resource b1) in
+  let delta = R.(A.array_resource b_first <*> A.array_resource b1) in
+  assume(R.inv full h ==> R.inv delta h);
   let x2 = RST.rst_frame
     (R.(A.array_resource b_first <*> A.array_resource b_second <*> A.array_resource b1))
     (fun _ -> (R.(A.array_resource b_first <*> A.array_resource b_second <*> A.array_resource b1)))
     (fun _ -> A.index b_second 0ul)
   in
 
-  let h = HST.get () in
-  assume((R.sel (A.array_view b_first) h).A.p = 0.5R);
-  assume((R.sel (A.array_view b_second) h).A.p = 0.5R);
-
+  let h' = HST.get () in
+  assume(R.sel (R.view_of delta) h == R.sel (R.view_of delta) h' ==>
+    R.sel (A.array_view b_first ) h == R.sel (A.array_view b_first) h' /\
+    R.sel (A.array_view b1 ) h == R.sel (A.array_view b1) h');
   RST.rst_frame
     (R.(A.array_resource b_first <*> A.array_resource b_second <*> A.array_resource b1))
     (fun _ -> R.(A.array_resource b <*> A.array_resource b1))
     (fun _ -> A.glue b b_first b_second);
 
-  let h = HST.get () in
-
-  assume((R.sel (A.array_view b) h).A.p = 0.5R);
-  assume((R.sel (A.array_view b1) h).A.p = 0.5R);
-  assume(Arr.mergeable b b1 /\ Arr.freeable b); // These ones have to be fixed in Lowstar.Array
-
+  let h'' = HST.get () in
   A.merge b b1;
   A.free b
